ver2/checker.v
@@ -1,0 +1,184 @@
+Require Import FORVES.program.
+Import Program.
+
+Require Import FORVES.stack_operation_instructions.
+Import StackOpInstrs.
+
+Require Import FORVES.execution_state.
+Import ExecutionState.
+
+Require Import FORVES.concrete_interpreter.
+Import ConcreteInterpreter.
+
+Require Import FORVES.optimizations_def.
+Import Optimizations_Def.
+
+Require Import FORVES.symbolic_execution.
+Import SymbolicExecution.
+
+Require Import FORVES.storage_ops_solvers.
+Import StorageOpsSolvers.
+
+Require Import FORVES.memory_ops_solvers.
+Import MemoryOpsSolvers.
+
+Require Import FORVES.symbolic_state_cmp.
+Import SymbolicStateCmp.
+
+Require Import FORVES.symbolic_execution_soundness.
+Import SymbolicExecutionSoundness.
+
+Require Import List.
+Import ListNotations.
+
+Module Checker.
+
+
+Definition checker_type := block -> block -> nat -> bool.
+
+
+Definition sem_eq_blocks (p1 p2: block) (k: nat) (ops: stack_op_instr_map) : Prop :=
+forall (in_st: state) (in_stk: stack),
+get_stack_st in_st = in_stk ->
+length in_stk = k ->
+exists (out_st : state),
+evm_exec_block_c p1 in_st ops = Some out_st /\
+evm_exec_block_c p2 in_st ops = Some out_st.
+
+
+Definition eq_block_chkr_snd (chkr : checker_type) : Prop :=
+forall (p1 p2: block) (k: nat),
+chkr p1 p2 k = true -> sem_eq_blocks p1 p2 k evm_stack_opm.
+
+
+Definition evm_eq_block_chkr'' (smem_updater: smemory_updater_type) 
+  (sstrg_updater: sstorage_updater_type) (mload_solver: mload_solver_type) 
+  (sload_solver: sload_solver_type) (fcmp: symbolic_state_cmp)
+  (opt: optim) (opt_p p: block) (k: nat) 
+  : bool :=
+match evm_sym_exec smem_updater sstrg_updater mload_solver sload_solver 
+      opt_p k evm_stack_opm with
+| None => false
+| Some sst_opt => 
+    match evm_sym_exec smem_updater sstrg_updater mload_solver sload_solver 
+            p k evm_stack_opm with 
+    | None => false
+    | Some sst_p => let (sst_opt', _) := opt sst_opt in 
+                    let (sst_p',   _) := opt sst_p in
+                    fcmp sst_p' sst_opt' evm_stack_opm
+                    (* Replace by other useful sound sst comparator or 
+                       a parameter + premise about its soundness *)
+    end
+end.
+
+Lemma equiv_checker''_correct: forall (opt_p p: block) 
+  (smem_updater: smemory_updater_type) (sstrg_updater: sstorage_updater_type) 
+  (mload_solver: mload_solver_type) (sload_solver: sload_solver_type)
+  (fcmp: symbolic_state_cmp)
+  (height: nat) (opt: optim) (in_es: state) (in_stk: stack),
+optim_snd opt ->
+smemory_updater_snd smem_updater ->
+sstorage_updater_snd sstrg_updater ->
+mload_solver_snd mload_solver ->
+sload_solver_snd sload_solver ->
+symbolic_state_cmp_snd fcmp ->
+evm_eq_block_chkr'' smem_updater sstrg_updater mload_solver 
+  sload_solver fcmp opt opt_p p height = true ->
+get_stack_st in_es = in_stk ->
+length in_stk = height ->
+exists (out_es_opt out_es_p: state),
+(evm_exec_block_c opt_p in_es evm_stack_opm = Some out_es_opt /\
+ evm_exec_block_c p in_es evm_stack_opm = Some out_es_p /\
+ get_stack_st out_es_opt = get_stack_st out_es_p /\
+ get_memory_st out_es_opt = get_memory_st out_es_p /\
+ get_storage_st out_es_opt = get_storage_st out_es_p /\ 
+ get_context_st out_es_opt = get_context_st out_es_p) (*trivial, ctx doesn't change*).
+Proof.
+intros opt_p p smem_updater sstrg_updater mload_solver sload_solver fcmp
+  height opt in_es in_stk Hopt_snd Hsmemory_upd Hstrg_upd Hmload_solver 
+  Hsload_solver Hcmp
+  Hchkr_true Hget_stk Hlen_stk.
+unfold evm_eq_block_chkr'' in Hchkr_true.
+destruct (evm_sym_exec smem_updater sstrg_updater mload_solver
+          sload_solver opt_p height evm_stack_opm) 
+            as [sst_opt|] eqn: eq_symb_exec_opt; try discriminate.
+destruct (evm_sym_exec smem_updater sstrg_updater mload_solver
+          sload_solver p height evm_stack_opm) 
+            as [sst_p|] eqn: eq_symb_exec_p; try discriminate.
+pose proof (symbolic_exec_snd smem_updater sstrg_updater mload_solver 
+  sload_solver opt_p height sst_opt evm_stack_opm Hsmemory_upd Hstrg_upd 
+  Hmload_solver Hsload_solver eq_symb_exec_opt) as [Hvalid_sst_opt Hconcr_opt'].
+rewrite <- Hget_stk in Hlen_stk.
+pose proof (Hconcr_opt' in_es Hlen_stk) as [out_es_opt [Hconcr_opt Hinst_sst_opt]].
+pose proof (symbolic_exec_snd smem_updater sstrg_updater mload_solver 
+  sload_solver p height sst_p evm_stack_opm Hsmemory_upd Hstrg_upd 
+  Hmload_solver Hsload_solver eq_symb_exec_p) as [Hvalid_sst Hconcr_p']. 
+pose proof (Hconcr_p' in_es Hlen_stk) as [out_es_p [Hconcr_p Hinst_sst]].
+exists out_es_opt. exists out_es_p.
+destruct (opt sst_p) as [sst_p' flag_p] eqn: eq_optimize_p.
+destruct (opt sst_opt) as [sst_opt' flag_opt] eqn: eq_optimize_popt.
+unfold st_is_instance_of_sst in Hinst_sst.
+destruct Hinst_sst as [out_es_p' [Heval_sst_p Heq_out_es_p]].
+apply eq_execution_states_ext in Heq_out_es_p.
+rewrite <- Heq_out_es_p in Heval_sst_p.
+unfold st_is_instance_of_sst in Hinst_sst_opt.
+destruct Hinst_sst_opt as [out_es_opt' [Heval_sst_opt Heq_out_es_opt]].
+apply eq_execution_states_ext in Heq_out_es_opt.
+rewrite <- Heq_out_es_opt in Heval_sst_opt.
+unfold optim_snd in Hopt_snd.
+pose proof (Hopt_snd sst_p sst_p' flag_p Hvalid_sst eq_optimize_p) as [_ Hp].
+pose proof (Hp in_es out_es_p Heval_sst_p) as Hevalp.
+pose proof (Hopt_snd sst_opt sst_opt' flag_opt Hvalid_sst_opt eq_optimize_popt)
+  as [_ Hopt].
+pose proof (Hopt in_es out_es_opt Heval_sst_opt) as Hevalopt.
+unfold symbolic_state_cmp_snd in Hcmp.
+pose proof (Hcmp sst_p' sst_opt' evm_stack_opm height Hchkr_true in_es Hlen_stk
+  ) as Heq_eval_sst_p_opt.
+rewrite -> Hevalopt in Heq_eval_sst_p_opt.
+rewrite -> Hevalp in Heq_eval_sst_p_opt.
+injection Heq_eval_sst_p_opt as eq_out_es.
+split; try split; try split; try split; try split.
+- assumption.
+- assumption.
+- rewrite -> eq_out_es. reflexivity.
+- rewrite -> eq_out_es. reflexivity.
+- rewrite -> eq_out_es. reflexivity.
+- rewrite -> eq_out_es. reflexivity.
+Qed.
+
+Theorem evm_eq_block_chkr''_snd: forall (opt: optim) 
+  (smem_updater: smemory_updater_type) (sstrg_updater: sstorage_updater_type) 
+  (mload_solver: mload_solver_type) (sload_solver: sload_solver_type)
+  (fcmp: symbolic_state_cmp), 
+optim_snd opt -> 
+smemory_updater_snd smem_updater ->
+sstorage_updater_snd sstrg_updater ->
+mload_solver_snd mload_solver ->
+sload_solver_snd sload_solver ->
+symbolic_state_cmp_snd fcmp ->
+eq_block_chkr_snd (evm_eq_block_chkr'' smem_updater 
+  sstrg_updater mload_solver sload_solver fcmp opt).
+Proof.
+intros opt smem_updater sstrg_updater mload_solver sload_solver fcmp Hopt_snd 
+  Hsmemory_upd Hstrg_upd Hmload_solver Hsload_solver Hcmp. 
+unfold eq_block_chkr_snd. intros p1 p2 k Hchecker_true.
+unfold sem_eq_blocks. intros in_st in_stk Hgetstk Hlenstk.
+pose proof (equiv_checker''_correct p1 p2 smem_updater sstrg_updater 
+  mload_solver sload_solver fcmp k opt in_st in_stk Hopt_snd
+  Hsmemory_upd Hstrg_upd Hmload_solver Hsload_solver Hcmp
+  Hchecker_true Hgetstk Hlenstk) 
+  as [out_es_opt [out_es [Hconcr_p1 [Hconcr_p2 Heq_states]]]].
+exists out_es.
+destruct in_st as [stack mem storage ctx] eqn: eq_in_st.
+destruct out_es as [stack_o mem_o storage_o ctx_o] eqn: eq_out_st.
+destruct out_es_opt as [stack_op mem_op storage_op ctx_op] eqn: eq_out_opt.
+simpl in Heq_states.
+destruct Heq_states as [Heq_stk [Heq_mem [Heq_strg Heq_ctx]]].
+rewrite -> Hconcr_p1. rewrite -> Hconcr_p2.
+rewrite -> Heq_stk. rewrite -> Heq_mem. 
+rewrite -> Heq_strg. rewrite -> Heq_ctx.
+auto.
+Qed.
+
+
+End Checker.
